Proved Cantor-Schroder-Bernstein!

Blerp/Basic.lean
@@ -1,1 +1,254 @@
-def hello := "world"
+inductive InX1 {X Y : Type u} (f : X → Y) (g : Y → X) : X → Prop
+    | base : ∀ x : X, (∀ y : Y, x ≠ g y) → InX1 f g x
+    | step : ∀ x : X, InX1 f g x → InX1 f g (g (f x))
+
+theorem CSB {A B : Type u} (f : A → B) (g : B → A) (hf : f.Injective) (hg : g.Injective) :
+    ∃ h : A → B, h.Injective ∧ h.Surjective := by
+/-
+    A1 is everything in A that stops in A when you pull back
+    same for B1 and B
+-/
+    let InA1 : A → Prop := InX1 f g
+    let InB1 : B → Prop := InX1 g f
+/-
+    A2 is everything in A that stops in B
+    B2 is everything in B that stops in A
+    A2 = g (B1) and B2 = f (A1)
+-/
+    let InA2 : A → Prop := fun a ↦ ∃ b : B, InB1 b ∧ a = g b
+    let InB2 : B → Prop := fun b ↦ ∃ a : A, InA1 a ∧ b = f a
+
+/-
+    A3 and B3 are everything else : infinite ascent
+-/
+
+    let InA3 : A → Prop := fun a ↦ ¬ InA1 a ∧  ¬ InA2 a
+    let InB3 : B → Prop := fun b ↦ ¬ InB1 b ∧  ¬ InB2 b
+
+/-
+I need to show that each a : A lies in exactly one of A1, A2, A3. lying in A3
+by definition means not being in A1 or A2; so I need to show that A1 and A2
+are mutually exclusive as well (same for B)
+-/
+
+    have not_A2_of_A1 : ∀ a : A, ¬ InA1 a ∨ ¬ InA2 a := by
+        simp only [Classical.or_iff_not_imp_left, Classical.not_not]
+        intro z hz; induction hz with
+        | base a ha =>
+            unfold InA2; simp only [not_exists, not_and]
+            intro b hb; exact ha b
+        | step a' ha'1 ha'2 =>
+            unfold InA2 at ha'2 ⊢
+            simp only [not_exists, not_and] at ha'2 ⊢
+            simp [Function.Injective.ne_iff hg]
+            intro y hy; induction hy with
+            |   base b hb =>
+                apply Ne.symm; exact hb a'
+            |   step b' hb'1 hb'2 =>
+                simp [Function.Injective.ne_iff hf]
+                exact ha'2 b' hb'1
+
+    have not_B2_of_B1 : ∀ b : B, ¬ InB1 b ∨ ¬ InB2 b := by
+        simp only [Classical.or_iff_not_imp_left, Classical.not_not]
+        intro z hz; induction hz with
+        | base b hb =>
+            unfold InB2; simp only [not_exists, not_and]
+            intro a ha; exact hb a
+        | step b' hb'1 hb'2 =>
+            unfold InB2 at hb'2 ⊢
+            simp only [not_exists, not_and] at hb'2 ⊢
+            simp [Function.Injective.ne_iff hf]
+            intro y hy; induction hy with
+            |   base a ha =>
+                apply Ne.symm; exact ha b'
+            |   step a' ha'1 ha'2 =>
+                simp [Function.Injective.ne_iff hg]
+                exact hb'2 a' ha'1
+
+/-
+    The basic trick now is that f is a bijection from A1 to B2, and from A3 to B3,
+    and g is a bijection from B1 to A2, so g⁻¹ is a bijection from A2 to B1.
+
+    we'll define φ : A → B that equals g⁻¹ on A2 and equals f everywhere else
+
+    just need to show each of the pieces is surjective and that each of their ranges
+    are what they should be
+
+    we have f : A1 → B2 is surjective by the definition of B2
+-/
+
+    have hf_A1_B2_surj : ∀ b : B, InB2 b → ∃ a : A, InA1 a ∧ b = f a := by
+        unfold InB2; exact fun _ h ↦ h
+
+    have hg_B1_A2_surj : ∀ a : A, InA2 a → ∃ b : B, InB1 b ∧ a = g b := by
+        unfold InA2; exact fun _ h ↦ h
+
+    have hpartA : ∀ a : A, ¬ InA1 a → ¬ InA2 a → InA3 a :=
+        fun _ ha1 ha2 ↦ ⟨ha1, ha2⟩
+
+    have hpartB : ∀ b : B, ¬ InB1 b → ¬ InB2 b → InB3 b :=
+        fun _ hb1 hb2 ↦ ⟨hb1, hb2⟩
+
+/-
+    f maps A2 onto B1 and A1 onto B2 (similar for g)
+-/
+    have hf_B1_of_A2 : ∀ a : A, InA2 a →  InB1 (f a) := by
+        intro a ha; unfold InA2 at ha
+        have ⟨b, hb, hb'⟩ := ha
+        have h := InX1.step (f:= g) (g:= f) b hb
+        rw [←hb'] at h; exact h
+
+    have hf_A1_of_B2 : ∀ b : B, InB2 b → InA1 (g b) := by
+        intro b hb; unfold InB2 at hb
+        have ⟨a, ha, ha'⟩ := hb
+        have h := InX1.step (f:= f) (g:= g) a ha
+        rw [←ha'] at h; exact h
+
+    have hg_A2_of_B1 : ∀ b : B, InB1 b → InA2 (g b) := fun b hb ↦ ⟨b, hb, rfl⟩
+    have hf_B2_of_A1 : ∀ a : A, InA1 a → InB2 (f a) := fun a ha ↦ ⟨a, ha, rfl⟩
+
+/-
+    Anything NOT in B1 is in the range of f
+-/
+    have hB1_cp : ∀ b : B, ¬ InB1 b → ∃ a : A, b = f a := by
+        intro b hb; apply Classical.byContradiction; intro h
+        simp at h; have h' := InX1.base (f := g) (g := f) b h
+        exact hb h'
+
+    have hA1_cp : ∀ a : A, ¬ InA1 a → ∃ b : B, a = g b := by
+        intro a ha; apply Classical.byContradiction; intro h
+        simp at h; have h' := InX1.base (f := f) (g := g) a h
+        exact ha h'
+
+/-
+    This shows that f is a bijection between A3 and B3, and similarly
+    g is a bijection between B3 and A3
+-/
+
+    have hf_A3_B3_surj : ∀ b : B, InB3 b → ∃ a : A, InA3 a ∧ b = f a := by
+        intro b hb; unfold InB3 at hb; obtain ⟨hb1, hb2⟩ := hb
+        unfold InB2 at hb2; simp only [not_exists, not_and] at hb2
+        have ⟨a, ha⟩  := hB1_cp b hb1; refine ⟨a, ?_, ha⟩
+        apply hpartA a
+        ·   intro ha1; exact hb2 a ha1 ha
+        ·   intro ha2; rw [ha] at hb1; exact hb1 (hf_B1_of_A2 a ha2)
+
+    have hg_B3_A3_surj : ∀ a : A, InA3 a → ∃ b : B, InB3 b ∧ a = g b := by
+        intro a ha; unfold InA3 at ha; obtain ⟨ha1, ha2⟩ := ha
+        unfold InA2 at ha2; simp only [not_exists, not_and] at ha2
+        have ⟨b, hb⟩  := hA1_cp a ha1; refine ⟨b, ?_, hb⟩
+        apply hpartB b
+        ·   intro hb1; exact ha2 b hb1 hb
+        ·   intro hb2; rw [hb] at ha1; exact ha1 (hf_A1_of_B2 b hb2)
+
+    have hf_B3_of_A3 : ∀ a : A, InA3 a → InB3 (f a) := by
+        intro a ha; have ⟨b, hb1, hb2⟩ := (hg_B3_A3_surj a ha)
+        rw [hb2]; apply hpartB
+        ·   generalize heq : f (g b) = y
+            intro hb'2; cases hb'2 with
+            | base z hz =>
+                exact (hz (g b)) heq.symm
+            | step z' hz' =>
+                rw [Function.Injective.eq_iff hf, Function.Injective.eq_iff hg] at heq
+                subst heq; unfold InB3 at hb1; exact hb1.1 hz'
+        ·   unfold InB2; simp only [not_exists, not_and]; intro x hx
+            simp only [Function.Injective.ne_iff hf]; intro hx'; subst hx'; rw [← hb2] at hx
+            unfold InA3 at ha; exact ha.1 hx
+
+    have hg_A3_of_B3 : ∀ b : B, InB3 b → InA3 (g b) := by
+        intro b hb; have ⟨a, ha1, ha2⟩ := (hf_A3_B3_surj b hb)
+        rw [ha2]; apply hpartA
+        ·   generalize heq : g (f a) = y
+            intro ha'2; cases ha'2 with
+            | base z hz =>
+                exact (hz (f a)) heq.symm
+            | step z' hz' =>
+                rw [Function.Injective.eq_iff hg, Function.Injective.eq_iff hf] at heq
+                subst heq; unfold InA3 at ha1; exact ha1.1 hz'
+        ·   unfold InA2; simp only [not_exists, not_and]; intro x hx
+            simp only [Function.Injective.ne_iff hg]; intro hx'; subst hx'; rw [← ha2] at hx
+            unfold InB3 at hb; exact hb.1 hx
+
+/-
+    f is NOT surjective from A2 onto B1; but g is bijective from B1 to A2, so I need to
+    invert it; this uses the axiom of choice to construct A function that goes backwards
+    then I show it's bijective by showing its composition with g gives the identity
+-/
+
+
+    let g_inv (a : A) (ha : InA2 a) : B := Exists.choose (hg_B1_A2_surj a ha)
+
+    have hg_g_inv : ∀ a : A, (ha : InA2 a) → g (g_inv a ha) = a := by
+        intro a ha; have ⟨_, h'⟩ := Exists.choose_spec (hg_B1_A2_surj a ha)
+        unfold g_inv; symm; exact h'
+
+/-
+    this actually shows g_inv is injective
+-/
+    have hg_inv_g : ∀ b : B, (hb : InB1 b) → (g_inv (g b) (hg_A2_of_B1 b hb) = b) := by
+        intro b hb; have ha : InA2 (g b) := hg_A2_of_B1 b hb
+        have h := hg_g_inv (g b) (ha)
+        rwa [Function.Injective.eq_iff hg] at h
+
+/-
+    this actually shows that g_inv is surjective
+-/
+
+    let φ : A → B := fun a ↦ by
+        by_cases h : InA2 a
+        ·   exact g_inv a h
+        exact f a
+
+/-
+    Putting it all together
+-/
+    refine ⟨φ, ?injective, ?surjective⟩
+    ·   intro x y hxy
+        unfold φ at hxy; split at hxy <;> split at hxy
+        ·   expose_names; rw [← hg_g_inv x h, ← hg_g_inv y h_1]
+            rwa [Function.Injective.eq_iff hg]
+        ·   expose_names; exfalso; have h' : InA1 y ∨ InA3 y := by
+                rw [Classical.or_iff_not_imp_left]
+                exact fun x ↦ hpartA y x h_1
+            rcases h' with ha | ha
+            ·   have hxy' := congrArg g hxy; rw [hg_g_inv x h] at hxy'
+                subst hxy'; have ⟨b', hb'1, hb'2⟩ := h
+                rw [Function.Injective.eq_iff hg] at hb'2
+                have hb'3 : InB2 b' := ⟨y, ha, hb'2.symm⟩
+                exact (Or.neg_resolve_left (not_B2_of_B1 b') hb'1) hb'3
+            ·   have hxy' := congrArg g hxy; rw [hg_g_inv x h] at hxy'
+                subst hxy'; have ⟨b', hb'1, hb'2⟩ := h
+                rw [Function.Injective.eq_iff hg] at hb'2
+                have hb'3 : InB3 (f y) := hf_B3_of_A3 y ha
+                rw [hb'2] at hb'3
+                unfold InB3 at hb'3; exact hb'3.1 hb'1
+        ·   expose_names; exfalso; have h' : InA1 x ∨ InA3 x := by
+                rw [Classical.or_iff_not_imp_left]
+                exact fun y ↦ hpartA x y h
+            rcases h' with ha | ha
+            ·   have hxy' := congrArg g hxy; rw [hg_g_inv y h_1] at hxy'
+                subst hxy'; have ⟨b', hb'1, hb'2⟩ := h_1
+                rw [Function.Injective.eq_iff hg] at hb'2
+                have hb'3 : InB2 b' := ⟨x, ha, hb'2.symm⟩
+                exact (Or.neg_resolve_left (not_B2_of_B1 b') hb'1) hb'3
+            ·   have hxy' := congrArg g hxy; rw [hg_g_inv y h_1] at hxy'
+                subst hxy'; have ⟨b', hb'1, hb'2⟩ := h_1
+                rw [Function.Injective.eq_iff hg] at hb'2
+                have hb'3 : InB3 (f x) := hf_B3_of_A3 x ha
+                rw [hb'2] at hb'3
+                unfold InB3 at hb'3; exact hb'3.1 hb'1
+        ·   rwa [Function.Injective.eq_iff hf] at hxy
+    ·   intro b; have hcases := hpartB b; simp [← Classical.or_iff_not_imp_left] at hcases
+        rcases hcases with h | h | h
+        ·   refine ⟨g b, ?_⟩
+            unfold φ; split
+            ·   expose_names; exact hg_inv_g b h
+            ·   expose_names; exact absurd ⟨b, h, rfl⟩ h_1
+        ·   obtain ⟨a, ha, ha'⟩ := h; refine ⟨a, ?_⟩
+            unfold φ; split
+            ·   expose_names; exact absurd h (Or.neg_resolve_left (not_A2_of_A1 a) ha)
+            ·   exact ha'.symm
+        ·   obtain ⟨a, ha, ha'⟩ := hf_A3_B3_surj b h; refine ⟨a, ?_⟩
+            unfold φ; split
+            ·   expose_names; unfold InA3 at ha; exact absurd h_1 ha.2
+            ·   exact ha'.symm
